Challenge/Modexp/Submission/Proofs/Memo/PCs.lean
@@ -18,3 +18,4 @@ import Challenge.Modexp.Submission.Proofs.Memo.PCs.T16
 import Challenge.Modexp.Submission.Proofs.Memo.PCs.T17
 import Challenge.Modexp.Submission.Proofs.Memo.PCs.T18
 import Challenge.Modexp.Submission.Proofs.Memo.PCs.T19
+import Challenge.Modexp.Submission.Proofs.Memo.PCs.T20
